Otbn/Examples/WideAddMem.v
@@ -1,0 +1,94 @@
+Require Import Coq.Strings.String.
+Require Import Coq.Lists.List.
+Require Import Coq.micromega.Lia.
+Require Import Coq.ZArith.ZArith.
+Require Import coqutil.Byte.
+Require Import coqutil.Map.Interface.
+Require Import coqutil.Map.Properties.
+Require Import coqutil.Map.Separation.
+Require Import coqutil.Map.SeparationLogic.
+Require Import coqutil.Semantics.OmniSmallstepCombinators.
+Require Import coqutil.Tactics.Tactics.
+Require Import coqutil.Word.Interface.
+Require Import coqutil.Word.Properties.
+Require Import coqutil.Z.PushPullMod.
+Require Import Otbn.Examples.WideAdd.
+Require Import Otbn.Model.Clobbers.
+Require Import Otbn.Model.ISA.
+Require Import Otbn.Model.Linker.
+Require Import Otbn.Model.Map.
+Require Import Otbn.Model.Semantics.
+Require Import Otbn.Model.SemanticsProperties.
+Require Import Otbn.Model.StraightlineStep.
+Require Import Otbn.Model.Zsimplify.
+Require Import Otbn.Model.SubstLets.
+Import ListNotations.
+Import Semantics.Coercions.
+Local Open Scope Z_scope.
+
+(*** Simple program that adds two 256-bit values from memory. ***)
+
+(* Code reference:
+
+     wide_add_mem:
+       li       x2, 2
+       li       x3, 3
+       bn.lid   x2, 0(x12)
+       bn.lid   x3, 0(x13)
+       bn,add   w2, w2, w3
+       bn.sid   x2, 0(x12)
+       ret
+ *)
+
+Section __.
+  Context {word32 : word.word 32} {word32_ok : word.ok word32}.
+  Context {word256 : word.word 256} {word256_ok : word.ok word256}.
+  Context {regfile : map.map reg word32} {regfile_ok : map.ok regfile}.
+  Context {wregfile : map.map wreg word256} {wregfile_ok : map.ok wregfile}.
+  Context {flagfile : map.map flag bool} {flagfile_ok : map.ok flagfile}.
+  Context {mem : map.map word32 byte} {mem_ok : map.ok mem}.
+  Add Ring wring32: (@word.ring_theory 32 word32 word32_ok).
+  Add Ring wring256: (@word.ring_theory 256 word256 word256_ok).
+  
+  Definition wide_add_mem_fn : otbn_function :=
+    ("wide_add_mem",
+      map.empty,
+      [ (Addi x2 x0 2 : insn);
+        (Addi x3 x0 3 : insn);
+        (Bn_lid x2 false x12 false  0 : insn);
+        (Bn_lid x3 false x13 false  0 : insn);
+        (Bn_add w2 w2 w3 0 FG0 : insn);
+        (Bn_sid x2 false x12 false  0 : insn);
+        (Ret : insn)])%string.
+
+
+  Lemma wide_add_mem_correct :
+    forall regs wregs flags dmem cstack lstack (a b : word256) pa pb Ra Rb,
+      is_word_aligned 32 pa = true ->
+      is_word_aligned 32 pb = true ->
+      word.unsigned pa + 32 < DMEM_BYTES ->
+      word.unsigned pb + 32 < DMEM_BYTES ->
+      map.get regs (gpreg x12) = Some pa ->
+      map.get regs (gpreg x13) = Some pb ->
+      (* note: the separation-logic setup does not require the operands to be disjoint *)
+      (word_at pa a * Ra)%sep dmem ->
+      (word_at pb b * Rb)%sep dmem ->
+      returns
+        (fetch:=fetch_ctx [wide_add_mem_fn])
+        "wide_add_mem"%string regs wregs flags dmem cstack lstack
+        (fun regs' wregs' flags' dmem' =>
+           (word_at pa (word.add a b) * Ra)%sep dmem'
+           /\ clobbers [flagM FG0; flagL FG0; flagZ FG0; flagC FG0] flags flags'
+           /\ clobbers [wdreg w2; wdreg w3] wregs wregs'
+           /\ clobbers [gpreg x2; gpreg x3] regs regs').
+  Proof.
+    cbv [wide_add_mem_fn returns]. intros; subst.
+    
+    repeat straightline_step.
+
+    eapply eventually_ret; [ reflexivity | eassumption | ].
+    ssplit; try reflexivity; [ | solve_clobbers .. ].
+    ecancel_assumption.
+  Qed.
+
+End __.
